Setlec/Kernel/CheckerC.lean
@@ -449,7 +449,7 @@ def checkIndDeclC (env : Env) (block : List ConstantInfo) : CheckM Env := do
         etaCtor := cvC.name, etaParams := nP, etaFields := nF,
         unitlike := checkUnitThmC env cvT.name cvT.levelParams nP,
         unitParams := nP,
-        ruleK := nF == 0 && piResultSortC cvT.type == some .zero }
+        ruleK := nF == 0 && piResultIsProp cvT.type }
     let env₂ ← block.foldlM
       (checkIndMemberC (block.map (·.name)) caps) env
     -- the whole projection name family must be ours to install
